hfc/FFAMemoryHypCall.v
@@ -6,26 +6,41 @@
     following files are relavant to this formalization. 
 
 - [FFAMemoryHypCallIntro.v]
-  - This file introduces several relavant concepts that are necessary in the FF-A
-    memory management interface formalization (e.g., FFA version number, identifiers in FFA) 
+  - This file introduces several concepts that are closely related to the FF-A
+    memory management interface. 
+    Other files that contain formal definitions rely on concepts that this file describes. 
+    Therefore, looking at this file may help readers understand our formal definitions. 
+
 - [FFAMemoryHypCallDescriptorState.v]
-  - This file introduces formal definitions of descriptor data structures. They are 
-    related to Sections 5.10, 5.11, and 5.12 in the document.
+  - This file contains formal definitions of descriptor data structures defined in
+    Sections 5.10, 5.11, and 5.12 of the FF-A document. 
+    Those descriptors contain several information that 
+    memory management hypervisor calls have to look at during its evaluations.
+
 - [FFAMemoryHypCallState.v]
-  - This file introduces abstract states of our formalizations.
+  - This file introduces the abstract state definition, the mathematical view of 
+    the entire system with hiding unnecessary details. 
+
 - [FFAMemoryHypCallCoreTransition.v]
-  - This file contains transition rules of FFA memory management interfaces. 
-  - Core transition rules in this file change ownership and accessibility information of the memory adress 
-    that interfaces want to handle.
+  - This file contains core transition rules of FFA memory management interfaces. 
+  - Core transition rules in this file change ownership and accessibility information 
+    of the memory adress that interfaces want to handle.
+
 - [FFAMemoryHypCallAdditionalStepsAuxiliaryFunctions.v]
+  - Auxiliary functions that makes the entire specifications more readable 
+    and structured.
+
 - [FFAMemoryHypCallAdditionalSteps.v]
-  - Other transition rules can be treated as wrappers of core transition rules
+  - Transition rules in this file can be treated as wrappers of core transition rules
     by adding several safety checks and/or invariants that the document contains.
-  - The relevant parts with this file in the FF-A document are Chapters 5 and 11.
+  - The relevant parts in the FF-A document are Chapters 5 and 11.
+
 - [FFAMemoryHypCallTestingInterface.v]
-  - This file provides testing interfaces (e.g., context switchings, dispatch, and so on).
+   - This file provides testing interfaces (e.g., context switchings, dispatch, and so on).
+
 - [FFAMemoryHypCallTesting.v]
   - This file provides test cases.
+
 - [FFAMemoryHypCallWellFormedProof.v]
   - This file contains the safety proof of our specifications, especially proofs
     related to well-formedness conditions that FFA memory management
