hfc/FFAMemoryHypCallCoreTransition.v
@@ -47,19 +47,25 @@ Require Export FFAMemoryHypCallState.
 (** *             Core Step Rules                            *)
 (*************************************************************)
 (** This file defines the core step rules of FFA memory management 
-    interfaces *)  
- 
+    interfaces *)
+
+(* begin hide *)
+
 Notation "'do' X <- A ;;; B" :=
   (match A with Some X => B |
            None => None
    end)
-    (at level 200, X ident, A at level 100, B at level 200) : ffa_monad_scope.
- 
+    (at level 200, X ident, A at level 100, B at level 200)
+  : ffa_monad_scope.
+
 Notation " 'check' A ;;; B" :=
   (if A then B else None)
-    (at level 200, A at level 100, B at level 200) : ffa_monad_scope.
+    (at level 200, A at level 100, B at level 200)
+  : ffa_monad_scope.
 
 Local Open Scope ffa_monad_scope.
+
+(* end hide *)
 
 (** Three roles in the FFA_XXX communications, and endpoints in the communications 
 
@@ -76,7 +82,7 @@ Local Open Scope ffa_monad_scope.
 
 (** 5.4.1 Ownership and access rules
    - There are invariants that we have to enforce 
-   *)
+ *)
 
 (*************************************************************)
 (** **            Valid Combinations                         *)
@@ -145,7 +151,6 @@ Section VALID_COMBINATIONS.
 
   Definition hyp_mem_local_props (st : AbstractState) :=
     st.(hypervisor_context).(mem_properties).(mem_local_properties).
-
   
 End VALID_COMBINATIONS.
 
@@ -267,41 +272,41 @@ Section FFA_MEMORY_INTERFACE_CORE_STEPS.
      *)
     
     Definition ffa_mem_donate_core_transition_spec
-               (lender borrower : ffa_UUID_t) (address: Z) (st: AbstractState)
+               (lender borrower : ffa_UUID_t) (page_number: Z) (st: AbstractState)
     : option (AbstractState * bool) :=
       (** - Find out memory properties *) 
-      do global_property <- ZTree.get address (hyp_mem_global_props st) ;;; 
+      do global_property <- ZTree.get page_number (hyp_mem_global_props st) ;;; 
       do lender_properties_pool <- ZTree.get lender (hyp_mem_local_props st) ;;;
       do borrower_properties_pool <- ZTree.get borrower (hyp_mem_local_props st) ;;;
-      do lender_property <- ZTree.get address lender_properties_pool ;;;
+      do lender_property <- ZTree.get page_number lender_properties_pool ;;;
       (** - check memory properties :
             - lender has to have onwership
             - lender has to have exclusive access to the address
             - borrower does not have the memory in its memory property pool 
        *)
       match global_property, lender_property,
-            ZTree.get address borrower_properties_pool  with
-      | mkMemGlobalProperties owned accessible _ _ _ dirty,
+            ZTree.get page_number borrower_properties_pool  with
+      | mkMemGlobalProperties is_ns owned accessible _ _ _ dirty,
         mkMemLocalProperties local_owned _ _ _, None =>
         (** - Check the valid onwership and accessibility combination for lender and borrower *)
-        match mem_states_valid_combination lender borrower owned accessible,
+        match is_ns, mem_states_valid_combination lender borrower owned accessible,
               owned, accessible, local_owned with
-        | true, Owned owner, ExclusiveAccess ex_accessor, LocalOwned =>
+        | false, true, Owned owner, ExclusiveAccess ex_accessor, LocalOwned =>
           if decide (owner = lender) && decide (ex_accessor = lender)
           then
             (** - Only change accessibility option of the lender. The remaining operations will
                 be performed in the retrieve *)
             let new_global_props :=
-                ZTree.set address (global_property {accessible_by: NoAccess})
+                ZTree.set page_number (global_property {accessible_by: NoAccess})
                           (hyp_mem_global_props st) in
             let new_st :=
                 st {hypervisor_context / mem_properties :
                       mkMemProperties new_global_props (hyp_mem_local_props st)}
                    {system_log: st.(system_log)
-                                     ++(SetAccessible lender address NoAccess)::nil} in
+                                     ++(SetAccessible lender page_number NoAccess)::nil} in
             Some (new_st, true)
           else Some (st, false)
-        | _, _, _, _ => Some (st, false)
+        | _, _, _, _, _ => Some (st, false)
         end
       | _, _, _ => Some (st, false)
       end.
@@ -315,14 +320,14 @@ Section FFA_MEMORY_INTERFACE_CORE_STEPS.
 
     Definition check_mem_states_valid_combination
                (lender : ffa_UUID_t) (borrower : ffa_UUID_t)
-               (address: Z) (st : AbstractState) :=
-      do global_property <- ZTree.get address (hyp_mem_global_props st) ;;;
+               (page_number: Z) (st : AbstractState) :=
+      do global_property <- ZTree.get page_number (hyp_mem_global_props st) ;;;
       do lender_properties_pool <- ZTree.get lender (hyp_mem_local_props st) ;;;
       do borrower_properties_pool <- ZTree.get borrower (hyp_mem_local_props st) ;;;
-      do lender_property <- ZTree.get address lender_properties_pool ;;;
+      do lender_property <- ZTree.get page_number lender_properties_pool ;;;
       match global_property, lender_property,
-            ZTree.get address borrower_properties_pool with
-      | mkMemGlobalProperties owned accessible _ _ _ dirty,
+            ZTree.get page_number borrower_properties_pool with
+      | mkMemGlobalProperties _ owned accessible _ _ _ dirty,
         mkMemLocalProperties local_owned _ _ _, None =>
         (** - Check the valid onwership and accessibility combination for lender and borrower *)        
         Some (mem_states_valid_combination lender borrower owned accessible)
@@ -331,20 +336,20 @@ Section FFA_MEMORY_INTERFACE_CORE_STEPS.
 
     Fixpoint check_mem_states_valid_combination_for_borrowers
              (lender : ffa_UUID_t) (borrowers : list ffa_UUID_t)
-             (address: Z) (st : AbstractState) :=
+             (page_number: Z) (st : AbstractState) :=
       match borrowers with
       | nil => Some true
       | hd::tl =>
-        do res <- check_mem_states_valid_combination_for_borrowers lender tl address st ;;;
-        check_mem_states_valid_combination lender hd address st
+        do res <- check_mem_states_valid_combination_for_borrowers lender tl page_number st ;;;
+        check_mem_states_valid_combination lender hd page_number st
       end.
 
     Definition check_mem_states_valid_combination_for_borrowers_unwrapper
              (lender : ffa_UUID_t) (borrowers : list ffa_UUID_t)
-             (address: Z) (st : AbstractState) :=
+             (page_number: Z) (st : AbstractState) :=
       (decide (length borrowers >= 1)%nat) && 
       match check_mem_states_valid_combination_for_borrowers lender borrowers
-                                                             address st with
+                                                             page_number st with
       | Some res => res
       | Non => false
       end.
@@ -390,15 +395,14 @@ Section FFA_MEMORY_INTERFACE_CORE_STEPS.
          calling the FFA_MEM_RECLAIM ABI (see 11.7 FFA_MEM_RECLAIM).
      *)
 
-
     Definition ffa_mem_lend_core_transition_spec
                (lender : ffa_UUID_t) (borrowers : list ffa_UUID_t)
-               (address: Z) (st : AbstractState)
+               (page_number: Z) (st : AbstractState)
     : option (AbstractState * bool) :=
       (** - Find out memory properties *) 
-      do global_property <- ZTree.get address (hyp_mem_global_props st) ;;;
+      do global_property <- ZTree.get page_number (hyp_mem_global_props st) ;;;
       do lender_properties_pool <- ZTree.get lender (hyp_mem_local_props st) ;;;
-      do lender_property <- ZTree.get address lender_properties_pool ;;;
+      do lender_property <- ZTree.get page_number lender_properties_pool ;;;
       (** - check memory properties :
             - lender has to have onwership
             - lender has to have exclusive access to the address
@@ -406,27 +410,27 @@ Section FFA_MEMORY_INTERFACE_CORE_STEPS.
        *)
       match global_property, lender_property,
             check_mem_states_valid_combination_for_borrowers_unwrapper
-              lender borrowers address st  with
-      | mkMemGlobalProperties owned accessible _ _ _ dirty,
+              lender borrowers page_number st  with
+      | mkMemGlobalProperties is_ns owned accessible _ _ _ dirty,
         mkMemLocalProperties local_owned _ _ _, true =>
         (** - Check the valid onwership and accessibility combination for lender and borrower *)        
-        match owned, accessible, local_owned with
-        | Owned owner, ExclusiveAccess ex_accessor, LocalOwned =>
+        match is_ns, owned, accessible, local_owned with
+        | false, Owned owner, ExclusiveAccess ex_accessor, LocalOwned =>
           if decide (owner = lender) && decide (ex_accessor = lender)
           then (** Only change accessibility option of the lender. The remaining operations will
                    be performed in the retrieve *)                 
                let new_global_props :=
                    ZTree.set
-                     address (global_property {accessible_by: NoAccess})
+                     page_number (global_property {accessible_by: NoAccess})
                      (hyp_mem_global_props st) in
                let new_st :=
                    st {hypervisor_context / mem_properties :
                          mkMemProperties new_global_props (hyp_mem_local_props st)}
                       {system_log: st.(system_log)
-                                        ++(SetAccessible lender address NoAccess)::nil} in                      
+                                        ++(SetAccessible lender page_number NoAccess)::nil} in                      
                Some (new_st, true)
           else Some (st, false)
-        | _, _, _ => Some (st, false)
+        | _, _, _, _ => Some (st, false)
         end
       | _, _, _ => Some (st, false)
       end.
@@ -472,12 +476,12 @@ Section FFA_MEMORY_INTERFACE_CORE_STEPS.
          calling the FFA_MEM_RECLAIM ABI (see 11.7 FFA_MEM_RECLAIM).
      *)
     Definition ffa_mem_share_core_transition_spec
-               (lender : ffa_UUID_t) (borrowers : list ffa_UUID_t) (address: Z) (st : AbstractState)
+               (lender : ffa_UUID_t) (borrowers : list ffa_UUID_t) (page_number: Z) (st : AbstractState)
     : option (AbstractState * bool) :=
       (** - Find out memory properties *) 
-      do global_property <- ZTree.get address (hyp_mem_global_props st) ;;;
+      do global_property <- ZTree.get page_number (hyp_mem_global_props st) ;;;
       do lender_properties_pool <- ZTree.get lender (hyp_mem_local_props st) ;;;
-      do lender_property <- ZTree.get address lender_properties_pool ;;;
+      do lender_property <- ZTree.get page_number lender_properties_pool ;;;
       (** - check memory properties :
             - lender has to have onwership
             - lender has to have exclusive access to the address
@@ -485,17 +489,17 @@ Section FFA_MEMORY_INTERFACE_CORE_STEPS.
        *)
       match global_property, lender_property,
             check_mem_states_valid_combination_for_borrowers_unwrapper
-              lender borrowers address st  with
-      | mkMemGlobalProperties owned accessible _ _ _ dirty,
+              lender borrowers page_number st  with
+      | mkMemGlobalProperties is_ns owned accessible _ _ _ dirty,
         mkMemLocalProperties local_owned _ _ _, true =>
         (** Check the valid onwership and accessibility combination for lender and borrower *)        
-        match owned, accessible, local_owned with
-        | Owned owner, ExclusiveAccess ex_accessor, LocalOwned =>
+        match is_ns, owned, accessible, local_owned with
+        | false, Owned owner, ExclusiveAccess ex_accessor, LocalOwned =>
           if decide (owner = lender) && decide (ex_accessor = lender)
           then (** Only change accessibility option of the lender. The remaining operations will
                    be performed in the retrieve *)                 
             let new_global_props :=
-                ZTree.set address
+                ZTree.set page_number
                           (global_property
                              {accessible_by: SharedAccess (lender::nil)})
                           (hyp_mem_global_props st) in
@@ -503,10 +507,10 @@ Section FFA_MEMORY_INTERFACE_CORE_STEPS.
                 st {hypervisor_context / mem_properties :
                       mkMemProperties new_global_props (hyp_mem_local_props st)}
                    {system_log: st.(system_log)
-                                     ++(SetAccessible lender address NoAccess)::nil} in                      
+                                     ++(SetAccessible lender page_number NoAccess)::nil} in                      
             Some (new_st, true)
           else Some (st, false)
-        | _, _, _ => Some (st, false)
+        | _, _, _, _ => Some (st, false)
         end
       | _, _, _ => Some (st, false)
       end.
@@ -553,44 +557,44 @@ Section FFA_MEMORY_INTERFACE_CORE_STEPS.
     (*************************************************************)    
 
     Definition ffa_mem_donate_retrieve_req_core_transition_spec
-               (lender borrower : ffa_UUID_t) (address: Z) (clean: bool) (st: AbstractState)
+               (lender borrower : ffa_UUID_t) (page_number: Z) (clean: bool) (st: AbstractState)
     : option (AbstractState * bool) :=
       (** - Find out memory properties *) 
-      do global_property <- ZTree.get address (hyp_mem_global_props st) ;;; 
+      do global_property <- ZTree.get page_number (hyp_mem_global_props st) ;;; 
       do lender_properties_pool <- ZTree.get lender (hyp_mem_local_props st) ;;;
       do borrower_properties_pool <- ZTree.get borrower (hyp_mem_local_props st) ;;;
-      do lender_property <- ZTree.get address lender_properties_pool ;;;
+      do lender_property <- ZTree.get page_number lender_properties_pool ;;;
       (** - check memory properties :
             - lender has to have onwership
             - lender has to have exclusive access to the address
             - borrower does not have the memory in its memory property pool 
        *)
       match global_property, lender_property,
-            ZTree.get address borrower_properties_pool  with
-      | mkMemGlobalProperties owned accessible _ _ _ dirty,
+            ZTree.get page_number borrower_properties_pool  with
+      | mkMemGlobalProperties is_ns owned accessible _ _ _ dirty,
         mkMemLocalProperties local_owned _ _ _, None =>
         (** - Check the valid onwership and accessibility combination for lender and borrower *)
-        match mem_states_valid_combination lender borrower owned accessible,
+        match is_ns, mem_states_valid_combination lender borrower owned accessible,
               owned, accessible, local_owned with
-        | true, Owned owner, NoAccess, LocalOwned =>
+        | false, true, Owned owner, NoAccess, LocalOwned =>
           if decide (owner = lender)
           then let new_dirty := if clean then MemClean else dirty in
                (** - Only change accessibility option of the lender. The remaining operations will
                      be performed in the retrieve *)
                let new_global_properties :=
-                   ZTree.set address
+                   ZTree.set page_number
                              (global_property
                                 {owned_by: Owned borrower}
                                 {accessible_by: ExclusiveAccess borrower}
                                 {mem_dirty : new_dirty}) (hyp_mem_global_props st) in
                (** - Remove the corresponding map in the lender memory local properties pool *)
                let new_lender_properties_pool :=
-                   ZTree.remove address lender_properties_pool in
+                   ZTree.remove page_number lender_properties_pool in
                (** - Create the new  memory local properties pool for the borrower.
                      Instead of making a new ini  tial state, we copied the previous local properties that lender had. 
                      Next opeartions can adjust th     e properties if it is necessary *)
                let new_borrower_properties_pool :=
-                   ZTree.set address
+                   ZTree.set page_number
                              (gen_own_mem_local_properties_wrapper lender_property) 
                              borrower_properties_pool in
                let new_local_properties_global_pool' :=
@@ -605,13 +609,13 @@ Section FFA_MEMORY_INTERFACE_CORE_STEPS.
                          mkMemProperties new_global_properties
                                          new_local_properties_global_pool}
                       {system_log: st.(system_log)
-                                        ++((SetOwner lender address (Owned borrower))
-                                             ::(SetAccessible lender address
+                                        ++((SetOwner lender page_number (Owned borrower))
+                                             ::(SetAccessible lender page_number
                                                              (ExclusiveAccess borrower))
-                                             ::(SetDirty lender address new_dirty)::nil)} in
+                                             ::(SetDirty lender page_number new_dirty)::nil)} in
                Some (new_st, true)
           else Some (st, false)
-        | _, _, _, _ => Some (st, false)
+        | _, _, _, _, _ => Some (st, false)
         end
       | _, _, _ => Some (st, false)
       end.
@@ -635,35 +639,35 @@ Section FFA_MEMORY_INTERFACE_CORE_STEPS.
     
     Definition ffa_mem_lend_retrieve_req_core_transition_spec
                (lender borrower : ffa_UUID_t) (borrower_num : Z)
-               (address: Z) (clean: bool) (st: AbstractState)
+               (page_number: Z) (clean: bool) (st: AbstractState)
     : option (AbstractState * bool) :=
       (** - Find out memory properties *) 
-      do global_property <- ZTree.get address (hyp_mem_global_props st) ;;;
+      do global_property <- ZTree.get page_number (hyp_mem_global_props st) ;;;
       do lender_properties_pool <- ZTree.get lender (hyp_mem_local_props st) ;;;
       do borrower_properties_pool <- ZTree.get borrower (hyp_mem_local_props st) ;;;
-      do lender_property <- ZTree.get address lender_properties_pool ;;;
+      do lender_property <- ZTree.get page_number lender_properties_pool ;;;
       (** - check memory properties :
             - lender has to have onwership
             - lender has to have exclusive access to the address
             - borrower does not have the memory in its memory property pool 
        *)
       match global_property, lender_property,
-            ZTree.get address borrower_properties_pool,
+            ZTree.get page_number borrower_properties_pool,
             decide (borrower_num >= 1)  with
-      | mkMemGlobalProperties owned accessible _ _ _ dirty,
+      | mkMemGlobalProperties is_ns owned accessible _ _ _ dirty,
         mkMemLocalProperties local_owned _ _ _, None, left _ =>
         (** - Check the valid onwership and accessibility combination for lender and borrower *)
-        match mem_states_valid_combination
+        match is_ns, mem_states_valid_combination
                 lender borrower owned accessible,
               owned, add_accessor borrower borrower_num accessible,
               local_owned with
-        | true, Owned owner, Some new_accessibility, LocalOwned =>
+        | false, true, Owned owner, Some new_accessibility, LocalOwned =>
           if decide (owner = lender)
           then let new_dirty := if clean then MemClean else dirty in
                (** - Only change accessibility option of the lender. The remaining operations will
                      be performed in the retrieve *)
                let new_global_properties :=
-                   ZTree.set address
+                   ZTree.set page_number
                              (global_property
                                 {owned_by: Owned borrower}
                                 {accessible_by: new_accessibility}
@@ -672,7 +676,7 @@ Section FFA_MEMORY_INTERFACE_CORE_STEPS.
                      Instead of making a new initial state, we copied the previous local properties that lender had. 
                      Next opeartions can adjust the properties if it is necessary *)
                let new_borrower_properties_pool :=
-                   ZTree.set address
+                   ZTree.set page_number
                              (gen_borrow_mem_local_properties_wrapper
                                 lender lender_property) 
                              borrower_properties_pool in
@@ -685,13 +689,13 @@ Section FFA_MEMORY_INTERFACE_CORE_STEPS.
                          mkMemProperties new_global_properties
                                          new_local_properties_global_pool}
                       {system_log: st.(system_log)
-                                        ++((SetOwner lender address (Owned borrower))
-                                             ::(SetAccessible lender address
+                                        ++((SetOwner lender page_number (Owned borrower))
+                                             ::(SetAccessible lender page_number
                                                              (ExclusiveAccess borrower))
-                                             ::(SetDirty lender address new_dirty)::nil)} in
+                                             ::(SetDirty lender page_number new_dirty)::nil)} in
                Some (new_st, true)
           else Some (st, false)
-        | _, _, _, _ => Some (st, false)
+        | _, _, _, _, _ => Some (st, false)
         end
       | _, _, _, _ => Some (st, false)
       end.
@@ -701,32 +705,32 @@ Section FFA_MEMORY_INTERFACE_CORE_STEPS.
     (*************************************************************)    
          
     Definition ffa_mem_share_retrieve_req_core_transition_spec
-               (lender borrower : ffa_UUID_t) (address: Z) (clean: bool) (st : AbstractState)
+               (lender borrower : ffa_UUID_t) (page_number: Z) (clean: bool) (st : AbstractState)
       : option (AbstractState * bool) :=
       (** - Find out memory properties *) 
-      do global_property <- ZTree.get address (hyp_mem_global_props st) ;;;
+      do global_property <- ZTree.get page_number (hyp_mem_global_props st) ;;;
       do lender_properties_pool <- ZTree.get lender (hyp_mem_local_props st) ;;;
       do borrower_properties_pool <- ZTree.get borrower (hyp_mem_local_props st) ;;;
-      do lender_property <- ZTree.get address lender_properties_pool ;;;
+      do lender_property <- ZTree.get page_number lender_properties_pool ;;;
       (** - check memory properties :
             - lender has to have onwership
             - lender has to have exclusive access to the address
             - borrower does not have the memory in its memory property pool 
        *)
       match global_property, lender_property,
-            ZTree.get address borrower_properties_pool  with
-      | mkMemGlobalProperties owned accessible _ _ _ dirty,
+            ZTree.get page_number borrower_properties_pool  with
+      | mkMemGlobalProperties is_ns owned accessible _ _ _ dirty,
         mkMemLocalProperties local_owned _ _ _, None =>
         (** - Check the valid onwership and accessibility combination for lender and borrower *)
-        match mem_states_valid_combination lender borrower owned accessible,
+        match is_ns, mem_states_valid_combination lender borrower owned accessible,
               owned, accessible, local_owned with
-        | true, Owned owner, SharedAccess accessors, LocalOwned =>
+        | is_ns, true, Owned owner, SharedAccess accessors, LocalOwned =>
           if decide (owner = lender) && (in_dec zeq lender accessors)
           then let new_dirty := if clean then MemClean else dirty in
                (** - Only change accessibility option of the lender. The remaining operations will
                      be performed in the retrieve *)
                let new_global_properties :=
-                   ZTree.set address
+                   ZTree.set page_number
                              (global_property
                                 {owned_by: Owned borrower}
                                 {accessible_by: SharedAccess (borrower::accessors)}
@@ -735,7 +739,7 @@ Section FFA_MEMORY_INTERFACE_CORE_STEPS.
                      Instead of making a new initial state, we copied the previous local properties that lender had. 
                      Next opeartions can adjust the properties if it is necessary *)
                let new_borrower_properties_pool :=
-                   ZTree.set address
+                   ZTree.set page_number
                              (gen_borrow_mem_local_properties_wrapper
                                 lender lender_property) 
                              borrower_properties_pool in
@@ -748,13 +752,13 @@ Section FFA_MEMORY_INTERFACE_CORE_STEPS.
                          mkMemProperties new_global_properties
                                          new_local_properties_global_pool}
                       {system_log: st.(system_log)
-                                        ++((SetOwner lender address (Owned borrower))
-                                             ::(SetAccessible lender address
+                                        ++((SetOwner lender page_number (Owned borrower))
+                                             ::(SetAccessible lender page_number
                                                              (SharedAccess (borrower::accessors)))
-                                             ::(SetDirty lender address new_dirty)::nil)} in
+                                             ::(SetDirty lender page_number new_dirty)::nil)} in
                Some (new_st, true)
           else Some (st, false)
-        | _, _, _, _ => Some (st, false)
+        | _, _, _, _, _ => Some (st, false)
         end
       | _, _, _ => Some (st, false)
       end.
@@ -838,32 +842,32 @@ Section FFA_MEMORY_INTERFACE_CORE_STEPS.
       end.
 
     Definition ffa_mem_relinquish_core_transition_spec
-               (lender borrower : ffa_UUID_t) (address: Z) (clean: bool) (st: AbstractState)
+               (lender borrower : ffa_UUID_t) (page_number: Z) (clean: bool) (st: AbstractState)
       : option (AbstractState * bool) :=
       (** - Find out memory properties *)
-      do global_property <- ZTree.get address (hyp_mem_global_props st) ;;;
+      do global_property <- ZTree.get page_number (hyp_mem_global_props st) ;;;
       do lender_properties_pool <- ZTree.get lender (hyp_mem_local_props st) ;;;
       do borrower_properties_pool <- ZTree.get borrower (hyp_mem_local_props st) ;;;
-      do lender_property <- ZTree.get address lender_properties_pool ;;;
+      do lender_property <- ZTree.get page_number lender_properties_pool ;;;
       (** - check memory properties :
             - lender has to have onwership
             - lender has to have exclusive access to the address
             - borrower does not have the memory in its memory property pool 
        *)
       match global_property, lender_property,
-            ZTree.get address borrower_properties_pool  with
-      | mkMemGlobalProperties owned accessible _ _ _ dirty,
+            ZTree.get page_number borrower_properties_pool  with
+      | mkMemGlobalProperties is_ns owned accessible _ _ _ dirty,
         mkMemLocalProperties local_owned _ _ _, None =>
         (** - Check the valid onwership and accessibility combination for lender and borrower *)
-        match mem_states_valid_combination lender borrower owned accessible,
+        match is_ns, mem_states_valid_combination lender borrower owned accessible,
               owned, remove_accessor lender borrower accessible, local_owned with
-        | true, Owned owner, Some new_accessibility, LocalOwned =>
+        | false, true, Owned owner, Some new_accessibility, LocalOwned =>
           if decide (owner = lender)
           then let new_dirty := if clean then MemClean else dirty in
                (** - Only change accessibility option of the lender. The remaining operations will
                      be performed in the retrieve *)
                let new_global_properties :=
-                   ZTree.set address (global_property
+                   ZTree.set page_number (global_property
                                         {owned_by: Owned lender}
                                         {accessible_by: new_accessibility}
                                         {mem_dirty : new_dirty}) (hyp_mem_global_props st) in
@@ -871,7 +875,7 @@ Section FFA_MEMORY_INTERFACE_CORE_STEPS.
                      Instead of making a new initial state, we copied the previous local properties that lender had. 
                      Next opeartions can adjust the properties if it is necessary *)               
                let new_borrower_properties_pool :=
-                   ZTree.remove address borrower_properties_pool in
+                   ZTree.remove page_number borrower_properties_pool in
                let new_local_properties_global_pool :=
                    ZTree.set borrower
                              new_borrower_properties_pool
@@ -881,21 +885,22 @@ Section FFA_MEMORY_INTERFACE_CORE_STEPS.
                          mkMemProperties new_global_properties
                                          new_local_properties_global_pool}
                       {system_log: st.(system_log)
-                                        ++((SetOwner lender address (Owned borrower))
-                                             ::(SetAccessible lender address new_accessibility)
-                                             ::(SetDirty lender address new_dirty)::nil)} in
+                                        ++((SetOwner lender page_number (Owned borrower))
+                                             ::(SetAccessible lender page_number new_accessibility)
+                                             ::(SetDirty lender page_number new_dirty)::nil)} in
                       
                Some (new_st, true)
           else Some (st, false)
-        | _, _, _, _ => Some (st, false)
+        | _, _, _, _, _ => Some (st, false)
         end
       | _, _, _ => Some (st, false)
       end.
 
   End FFA_MEM_RELINQUISH_CORE_STEPS.
 
-  (* - For FFA_MEM_RETRIEVE_RESP and FFA_MEM_RECLAIM, the memory state won't be changed. 
+(* - For FFA_MEM_RETRIEVE_RESP and FFA_MEM_RECLAIM, the memory state won't be changed. 
      FFA_MEM_RETRIEVE_RESP is the return value of RRA_MEM_RETRIEVE_REQ, and FFA_MEM_RECLAIM 
      is the mssage to trigger FFA_MEM_RELINQUISH. *)
   
 End FFA_MEMORY_INTERFACE_CORE_STEPS.
+
